qos, dup, retain refacta and add qos testcode

src/testErrorHandle.fst
@@ -14,27 +14,6 @@ module U8 = FStar.UInt8
 inline_for_extraction noextract
 let (!$) = C.String.of_literal
 
-val remaining_length_error_check1: u:unit -> St unit
-let remaining_length_error_check1 u =
-    let request: B.buffer U8.t = B.malloc HyperStack.root 0uy 5ul in
-        request.(0ul) <- 0x30uy;
-        request.(1ul) <- 0xD4uy;
-        request.(2ul) <- 0x01uy;
-        request.(3ul) <- 0x00uy;
-        request.(4ul) <- 0x0Auy;
-
-    let s : struct_fixed_header = parse request 5ul in
-        T.eq_str !$"remaining_length error check1" !$"remaining_length is invalid." s.error_message;
-B.free request
-
-val remaining_length_error_check2: u:unit -> St unit
-let remaining_length_error_check2 u =
-    let request: B.buffer U8.t = B.malloc HyperStack.root 0uy 1ul in
-
-    let s : struct_fixed_header = parse request 1ul in
-        T.eq_str !$"remaining_length error check2" !$"remaining_length is invalid." s.error_message;
-B.free request
-
 val message_type_error_check: u:unit -> St unit
 let message_type_error_check u =
     let request: B.buffer U8.t = B.malloc HyperStack.root 0uy 4ul in
@@ -119,16 +98,69 @@ let invalid_unsuback_flag_check u =
         T.eq_str !$"unsuback flag is invalid" !$"flag is invalid." s.error_message;
 B.free request
 
+val remaining_length_error_check1: u:unit -> St unit
+let remaining_length_error_check1 u =
+    let request: B.buffer U8.t = B.malloc HyperStack.root 0uy 5ul in
+        request.(0ul) <- 0x30uy;
+        request.(1ul) <- 0xD4uy;
+        request.(2ul) <- 0x01uy;
+        request.(3ul) <- 0x00uy;
+        request.(4ul) <- 0x0Auy;
+
+    let s : struct_fixed_header = parse request 5ul in
+        T.eq_str !$"remaining_length error check1" !$"remaining_length is invalid." s.error_message;
+B.free request
+
+val remaining_length_error_check2: u:unit -> St unit
+let remaining_length_error_check2 u =
+    let request: B.buffer U8.t = B.malloc HyperStack.root 0uy 1ul in
+
+    let s : struct_fixed_header = parse request 1ul in
+        T.eq_str !$"remaining_length error check2" !$"remaining_length is invalid." s.error_message;
+B.free request
+
+val invalid_qos_flag_check: u:unit -> St unit
+let invalid_qos_flag_check u =
+    let request = B.malloc HyperStack.root 0uy 24ul in
+        request.(0ul) <- 0x3Fuy;
+        request.(1ul) <- 0x16uy;
+        request.(2ul) <- 0x00uy;
+        request.(3ul) <- 0x0Auy;
+        request.(4ul) <- 0x74uy;
+        request.(5ul) <- 0x65uy;
+        request.(6ul) <- 0x73uy;
+        request.(7ul) <- 0x74uy;
+        request.(8ul) <- 0x2Fuy;
+        request.(9ul) <- 0x74uy;
+        request.(10ul) <- 0x6Fuy;
+        request.(11ul) <- 0x70uy;
+        request.(12ul) <- 0x69uy;
+        request.(13ul) <- 0x63uy;
+        request.(14ul) <- 0x68uy;
+        request.(15ul) <- 0x65uy;
+        request.(16ul) <- 0x6Cuy;
+        request.(17ul) <- 0x6Cuy;
+        request.(18ul) <- 0x6Fuy;
+        request.(19ul) <- 0x20uy;
+        request.(20ul) <- 0x6Duy;
+        request.(21ul) <- 0x71uy;
+        request.(22ul) <- 0x74uy;
+        request.(23ul) <- 0x74uy;
+    let s : struct_fixed_header = parse request 24ul in
+        T.eq_str !$"invalid qos flag check" !$"qos_flag is invalid." s.error_message;
+    B.free request
+
 val main : u:unit -> St C.exit_code
 let main () =
     T.test_start !$"TestErrorHandle";
-    remaining_length_error_check1 ();
-    remaining_length_error_check2 ();
     message_type_error_check ();
     invalid_pubrel_flag_check ();
     invalid_subscribe_flag_check ();
     invalid_unsubscribe_flag_check ();
     invalid_unsuback_flag_check ();
+    remaining_length_error_check1 ();
+    remaining_length_error_check2 ();
+    invalid_qos_flag_check ();
 
     T.test_end ();
     C.EXIT_SUCCESS
